theories/DecisionProcedure.v
@@ -1,0 +1,1409 @@
+Require Import CSL.IterativeContract.
+Require Import CSL.IterativeEquations.
+Require Import Setoid.
+Require Import Init.Tauto btauto.Btauto.
+Require Import Bool.Bool  Bool.Sumbool.
+Require Import Lists.List.
+Import ListNotations.
+Require Import Bool.Bool.
+Require Import micromega.Lia.
+From Equations Require Import Equations.
+(*******************************************************************************************************)
+Set Implicit Arguments.
+
+Section member.
+  Variable A : Set.
+  Hypothesis equals : A -> A -> bool.
+  
+  Fixpoint member (c : A) (l : list A) :=
+  match l with
+  | [] => false
+  | a::l' => equals a c || member c l' 
+  end.
+End member.
+
+Definition inclb (l0 l1 : list Contract) :bool := 
+ forallb (fun c0 => existsb (fun c1 => if Contract_eq_dec c0 c1 then true else false) l1) l0.
+
+Lemma inclb_iff : forall (l0 l1 : list Contract), inclb l0 l1 = true <-> incl l0 l1.
+Proof. unfold inclb. unfold incl. split. 
+- intros. rewrite forallb_forall in H. apply H in H0. rewrite existsb_exists in H0. destruct H0 as [x [P0 P1]].
+destruct (Contract_eq_dec a x).
+  * subst. assumption.
+  * discriminate.
+- intros. rewrite forallb_forall. intros. apply H in H0. rewrite existsb_exists. exists x. split.
+  * assumption.
+  * destruct (Contract_eq_dec x x).
+    ** reflexivity.
+    ** contradiction. 
+Qed.
+
+
+Lemma incl_reflect : forall (l0 l1 : list Contract), reflect (incl l0 l1) (inclb l0 l1).
+Proof. 
+intros. destruct (inclb l0 l1) eqn:Heqn.
+- constructor. rewrite inclb_iff in Heqn. assumption.
+- constructor. intro H. rewrite <- inclb_iff in H. rewrite Heqn in H. discriminate.
+Qed.
+
+
+
+Equations trace_derive (c : Contract) (s : Trace) : Contract :=
+trace_derive c [] := c;
+trace_derive c (e::s') := trace_derive (c/e) s'.
+Global Transparent trace_derive.
+Definition contains_all_derivatives_of c (l : list Contract) := forall (s : Trace), In (trace_derive c s) l.
+
+
+(*
+Inductive Trace_Derive : Contract -> Trace -> Contract -> Prop :=
+| Trace_Derive_Nil c : Trace_Derive c [] c
+| Trace_Derive_Cons c s c' e (H: Trace_Derive (c/e) s c') : Trace_Derive c (e::s) c'. (*rule motivated by constructor being analgous to cons on lists*)
+Hint Constructors Trace_Derive : coDB.*)
+
+Ltac autodp := auto with dpDB.
+Ltac eautodp := eauto with dpDB.
+
+(*
+Lemma derive_trace_derive : forall (c : Contract)(s : Trace)(e :EventType), trace_derive c (s++[e]) = (trace_derive c s) / e.
+Proof.
+intros. generalize dependent c. induction s;simpl;auto.
+Qed.*)
+(*
+Lemma trace_derive_spec : forall (c c' : Contract)(s : Trace), (trace_derive c s) = c' <-> Trace_Derive c s c'.
+Proof.
+split;intros.
+- funelim (trace_derive c s);simpl;auto with coDB.
+- induction H;auto. 
+Qed.*)
+
+Hint Resolve in_eq in_cons : core.
+
+Definition alphabet := [Notify;Transfer].
+Lemma in_alphabet : forall (e : EventType), In e alphabet.
+Proof.
+intros. unfold alphabet; destruct e; auto. 
+Qed.
+Global Opaque alphabet.
+
+Definition In_mod_R (c : Contract) (l : list Contract) := exists c', c' =R= c /\ In c' l.
+
+Lemma In_mod_R_eq : forall c l, In_mod_R c (c :: l).
+Proof.
+intros. exists c;auto.
+Qed.
+
+Lemma In_mod_R_cons : forall c c' l, In_mod_R c l -> In_mod_R c (c' :: l).
+Proof.
+intros. unfold In_mod_R in *. destruct_ctx. exists x. split;auto.
+Qed.
+
+Hint Resolve In_mod_R_eq In_mod_R_cons : dpDB.
+
+ 
+
+
+CoInductive AllDerivatives : Contract -> list Contract -> Prop :=
+| AD_fix c l (H0: forall e, AllDerivatives (c/e) l) (H1 : In c l)  : AllDerivatives c l
+| AD_sub c0 c1 l (H0: c0 =R= c1) (H1: AllDerivatives c0 l)  : AllDerivatives c1 l. (*Report: Necessary constructor for substitution because of Coq's guardedness constraint*)
+
+
+(*
+Inductive OnlyDerivatives : Contract -> list Contract -> Prop :=
+| OD_nil c : OnlyDerivatives c [c]
+| OD_cons c c' l e (H: In_mod_R c' l) (H1: OnlyDerivatives c 
+*)
+(*
+Lemma In_AllDerivatives_i_Trace_Derive : forall (c: Contract)(l : list Contract), 
+AllDerivatives c l -> (forall (s : Trace)(c_der : Contract), Trace_Derive c s c_der -> exists c', c' =R= c_der /\ In c' l).
+Proof.
+intros. generalize dependent c. induction s;intros.
+- inversion H0. subst. inversion H. destruct_ctx. exists x;auto.
+- inversion H0. inversion H. subst. eapply IHs. eapply H6. eauto.
+Qed.
+
+Lemma Trace_Derive_i_In_AllDerivatives : forall (c: Contract)(l : list Contract), 
+(forall (s : Trace)(c_der : Contract), Trace_Derive c s c_der -> exists c', c' =R= c_der /\ In c' l) -> AllDerivatives c l.
+Proof.
+cofix H_co.
+intros. constructor.
+- intros. apply H_co. intros. eapply H. constructor. eauto.
+- eauto with coDB.
+Qed.
+
+Theorem AllDerivatives_iff : forall (c: Contract)(l : list Contract), 
+AllDerivatives c l <-> (forall (s : Trace)(c_der : Contract), Trace_Derive c s c_der -> exists c', c' =R= c_der /\ In c' l).
+Proof.
+split;intros. 
+- eapply In_AllDerivatives_i_Trace_Derive;eauto.
+- eapply Trace_Derive_i_In_AllDerivatives;eauto.
+Qed.*)
+
+Lemma AllDerivatives_Failure : AllDerivatives Failure [Failure].
+Proof.
+cofix IH. constructor;auto;simpl;auto.
+Qed.
+
+Hint Resolve AllDerivatives_Failure : dpDB.
+
+
+
+Lemma AllDerivatives_cons : forall (c c_der : Contract)(l : list Contract), AllDerivatives c l -> AllDerivatives c (c_der::l).
+Proof.
+cofix IH.
+intros. inversion H. 
+- constructor;auto. 
+- eapply AD_sub. eauto. apply IH. auto.
+Qed.
+
+Hint Resolve AllDerivatives_cons : dpDB.
+
+(*
+Lemma AllDerivatives_derive : forall c l e, AllDerivatives c l -> AllDerivatives (c/e) l.
+Proof.
+cofix IH. intros. inversion H.
+- destruct_ctx.
+constructor; autodp. specialize H0 with e. destruct H0. auto.
+Qed.*)
+
+Lemma AllDerivatives_Success : AllDerivatives Success [Success;Failure].
+Proof.
+constructor; autodp.
+Qed.
+
+
+Hint Resolve AllDerivatives_Success : dpDB.
+
+Ltac eq_event_destruct :=
+  repeat match goal with
+         | [ |- context[if EventType_eq_dec ?e ?e then _ else _] ] => destruct (EventType_eq_dec e e);try contradiction
+         | [ |- context[if EventType_eq_dec ?e ?e0 then _ else _] ] => destruct (EventType_eq_dec e e0)
+         end.
+
+Lemma AllDerivatives_Event : forall (e : EventType), AllDerivatives (Event e) [Event e;Success;Failure].
+Proof.
+cofix IH.
+intros.
+constructor; intros;simpl.
+- eq_event_destruct; autodp. 
+- now left.
+Qed.
+
+Hint Resolve AllDerivatives_Event : dpDB.
+
+Definition plus_prod (l0 l1 : list Contract) :=
+match l0,l1 with
+| [],_ => l1
+| _,[] => l0
+|_,_ =>  map (fun p => (fst p) _+_ (snd p)) (list_prod l0 l1)
+end.
+
+Equations n_prod (ll : list (list Contract)) : list Contract by wf (length ll) lt :=
+n_prod [] := [];
+n_prod (l::[]) := l;
+n_prod (l::ll') := plus_prod l (n_prod (ll')).
+
+Global Transparent n_prod.
+
+Hint Unfold plus_prod : core.
+
+Fixpoint flatten (c : Contract) : list Contract :=
+match c with
+| c0 _+_ c1 => (flatten c0) ++ (flatten c1)
+| _ => [c]
+end.
+
+Lemma concat_n_prod : forall l ls, n_prod (l::ls) = plus_prod l ((n_prod ls)).
+Proof.
+intros. funelim (n_prod (l::ls)). simp n_prod. destruct l;auto.
+rewrite H. auto.
+Qed.
+
+Lemma in_n_prod : forall c0 c1 l0 l1, In c0 l0 -> In c1 l1 -> In (c0 _+_ c1) (n_prod [l0; l1]).
+Proof. Admitted.
+
+Inductive List_AllDerivatives : list Contract -> list (list Contract) -> Prop :=
+| List_AllDerivatives_nil : List_AllDerivatives [] []
+| List_AllDerivatives_cons c l cs ls (H0 : AllDerivatives c l) (H1 : List_AllDerivatives cs ls) : List_AllDerivatives (c::cs) (l::ls).
+
+Hint Constructors List_AllDerivatives : coDB.
+
+Lemma AllDerivatives_Flatten_iff : forall l ll, List_AllDerivatives l ll <-> AllDerivatives (plus_fold l) (n_prod ll).
+Proof. Admitted.
+
+
+
+Lemma flatten_non_empty : forall (c:Contract), exists c' l, flatten c = c'::l.
+Proof.
+induction c;intros.
+- exists Success. exists []. auto.
+- exists Failure. exists []. auto.
+- exists (Event e). exists []. auto.
+- destruct_ctx. exists x1. exists (x2 ++ (flatten c2)).
+  simpl. rewrite H0. now simpl.
+- exists (c1 _;_ c2). exists []. now simpl.
+- exists (Star c). exists []. now simpl.
+Qed.
+
+
+Lemma flatten_seq_derivative : forall c0 c1 e, flatten ((c0 _;_ c1)/ e) = [c0/e _;_ c1;o(c0)_;_(c1/e)].
+Proof.
+intros. now simpl.
+Qed.
+
+Lemma flatten_seq_trace_derive : forall s c0 c1 e, flatten ((c0 _;_ c1)// (e::s)) = flat_map (fun c => flatten (c//s)) (flatten ((c0 _;_ c1)/e)). 
+Proof.
+induction s;intros. now simpl. simpl. rewrite derive_plus. simpl.
+rewrite derive_plus. simpl. rewrite derive_plus. simpl.
+rewrite app_nil_r. auto.
+Qed.
+
+
+
+Lemma Failure_trace_derive : forall s, Failure//s = Failure.
+Proof.
+induction s;intros;auto.
+Qed.
+
+Hint Immediate o_derive Failure_trace_derive : dpDB.
+
+Lemma o_or : forall (c : Contract), o c = Success \/ o c = Failure.
+Proof.
+intros. o_destruct. rewrite H. now left. rewrite H. now right.
+Qed.
+
+
+Theorem flatten_seq_derive_shape : forall s c0 c1, exists l, (flatten ((c0 _;_ c1) // s)) = ((c0 // s) _;_ c1):: l /\
+ Forall (fun c => exists c' s, c = (o c') _;_ (c1//s)) l.
+Proof.
+induction s;intros.
+- simpl. exists []. split;auto.
+- rewrite flatten_seq_trace_derive. rewrite flatten_seq_derivative. simpl.
+  rewrite app_nil_r. specialize IHs with (c0/a) c1 as IHs'.
+  specialize IHs with (o c0) (c1/a). destruct_ctx. rewrite H1. rewrite H.
+  exists (x ++ o c0 // s _;_ c1 / a :: x0). split;auto.
+  rewrite Forall_forall in *. intros. apply in_app_or in H3. destruct H3.
+  * apply H0 in H3. destruct_ctx. exists x2. now exists x3.
+  * simpl in H3. destruct H3. 
+    ** rewrite <- H3. destruct (o_or c0).
+      *** rewrite H4. destruct s.
+        **** simpl. exists Success. now exists [a].
+        **** simpl. rewrite Failure_trace_derive. exists Failure. 
+             now exists [a].
+      *** rewrite H4. rewrite Failure_trace_derive. exists Failure.
+          now exists [a].
+    ** apply H2 in H3. destruct_ctx. rewrite H3.
+       exists x2. now exists (a::x3).
+Qed.
+
+
+Inductive Flat_Seq_Derivative : Contract -> Contract -> list Contract -> Prop :=
+| FSD_Single c0 c1 s : Flat_Seq_Derivative c0 c1 [c0//s _;_ c1]
+| FSD_Cons_S c0 c1 l s (H: Flat_Seq_Derivative c0 c1 l) : Flat_Seq_Derivative c0 c1 ((Success _;_(c1//s))::l)
+| FSD_Cons_F c0 c1 l s (H: Flat_Seq_Derivative c0 c1 l) : Flat_Seq_Derivative c0 c1 ((Failure _;_(c1//s))::l).
+
+(*
+Inductive Flat_Seq_Derivative : Contract -> Contract -> list Contract -> Prop :=
+| FSD_Single c0 c1 c_der0 l0  (H0: OnlyDerivatives c0 l0) 
+                              (H1: In_mod_R c_der0 l0) : Flat_Seq_Derivative c0 c1 [c_der0  _;_ c1]
+| FSD_Cons c0 c1 l0 l1 l_der c_der1 (H0: OnlyDerivatives c1 l1) 
+                                    (H1: In_mod_R c_der1 l1) 
+                                    (H2: Flat_Seq_Derivative c0 c1 l0 l_der) (H0: OnlyDerivatives c0 l0) (H2: In_mod_R c_der0 l0)(H1: In_mod_R c_der1 (Failure::l1)) : Flat_Seq_Derivative c0 c1 l0 l1 (c_der1::l_der).
+
+Inductive Flat_Seq_Derivative : Contract -> Contract -> list Contract -> list Contract -> list Contract -> Prop :=
+| FSD_Single c0 c1 l0 l1 c_der0 (H0: AllDerivatives c0 l0) (H1: AllDerivatives c1 l1) (H2: In_mod_R c_der0 l0): Flat_Seq_Derivative c0 c1 l0 l1 [c_der0  _;_ c1]
+| FSD_Cons c0 c1 l0 l1 l_der c_der1 (H: Flat_Seq_Derivative c0 c1 l0 l1 l_der) (H1: In_mod_R c_der1 (Failure::l1)) : Flat_Seq_Derivative c0 c1 l0 l1 (c_der1::l_der).*)
+(*
+Lemma in_share_AllDerivatives: forall c0 c l0 , AllDerivatives c0 l0 -> In_mod_R c l0 -> AllDerivatives c l0.
+Proof.
+cofix IH.
+intros. constructor.
+- intros. inversion H. eapply IH;auto. apply H. 
+
+Lemma in_AllDerivatives: forall c0 l0 c e, AllDerivatives c0 l0 -> In_mod_R c l0 -> In_mod_R (c/e) l0.
+Proof.
+intros. unfold In_mod_R in H0. destruct_ctx. inversion H. unfold In_mod_R in *)
+
+Lemma helper : forall s c0 e, (c0 // s) / e = c0 // (s ++ [e]).
+Proof.
+induction s;intros. now simpl.
+simpl. now rewrite IHs.
+Qed.
+
+Lemma helper2  : forall c e, c/e = c//[e].
+Proof. auto. Qed.
+
+Lemma flatten_cons : forall c, exists c' l, c'::l = flatten c .
+Proof. Admitted.
+
+(*
+Lemma seq_o_derivative_shape: forall c0 c1 s , Forall (fun c2 : Contract => exists s' : Trace, c2 = Failure _;_ c1 // s' \/ c2 = Success _;_ c1 // s')
+  (flatten ((o c0 _;_ c1) // s)).
+Proof.
+induction s;intros.
+- simpl. rewrite Forall_forall. intros. simpl in H. destruct H;try contradiction.
+  rewrite <- H. exists []. o_destruct. rewrite H0. now right.
+  rewrite H0. now left.
+- simpl. rewrite derive_plus. simpl. rewrite Forall_app. split;auto.*)
+
+Lemma seq_derivative_shape : forall (s : Trace)(c0 c1 : Contract) c l, c::l = flatten ((c0 _;_ c1)//s) -> c = c0//s _;_c1 /\ 
+Forall (fun (c : Contract) => exists (s' : Trace), c = Failure _;_ c1//s' \/ c = Success _;_ c1//s') l. 
+Proof.
+induction s;intros;simpl in *.
+- inversion H. split;auto.
+- rewrite derive_plus in H. simpl in H. destruct (flatten_cons (((c0 / a _;_ c1) // s))).
+  destruct H0. Search (_ ++ _ = _ -> _). rewrite <- H0 in H. simpl in H.
+  inversion H. apply IHs in H0. destruct H0. split;auto. 
+  rewrite Forall_app. split;auto.
+  
+ subst.
+induction l;intros. split.
+- destruct s. simpl in *. inversion H. auto. simpl in H.
+  rewrite derive_plus in H. simpl in H.
+  destruct (flatten_cons ((c0 / e _;_ c1) // s)).
+  destruct (flatten_cons (((o c0 _;_ c1 / e) // s))). destruct_ctx.
+  rewrite H0 in H. rewrite H1 in H. simpl in H. inversion H.
+  Search ([] = _). apply app_cons_not_nil in H4. contradiction.
+- auto.
+- split.
+  * simpl in H.
+ destruct s. simpl in H. inversion H. subst.
+
+ simpl in H4.
+  discriminate. inversion H4.
+  subst.
+ destruct (flatten ((c0 / e _;_ c1) // s)). inversion H.
+induction s;intros.
+- simpl. exists (c0 _;_ c1). exists []. split;auto.
+- simpl. rewrite derive_plus. simpl.
+  specialize IHs with (c0/a) c1.
+  destruct_ctx. exists x. exists (x0 ++ (flatten ((o c0 _;_ c1 / a) // s))).
+  split;auto.
+  * now rewrite <- H.
+  * split;auto. simpl. pose proof H1. rewrite Forall_forall in H1. rewrite Forall_forall.
+    intros. apply in_app_or in H3. destruct H2.
+    ** apply H1 in H2. auto.
+    **
+       eapply IHs. auto_rwd.
+
+Lemma Flat_Seq_Derivative_closed : forall c0 c1 l, Forall (fun c => Failure _;_ ) l exists s, c0 c1 l -> 
+Flat_Seq_Derivative c0 c1 (flat_map (fun c => flatten (c/e)) l).
+Proof.
+
+Lemma Flat_Seq_Derivative_closed : forall c0 c1 l e, Flat_Seq_Derivative c0 c1 l -> 
+Flat_Seq_Derivative c0 c1 (flat_map (fun c => flatten (c/e)) l).
+Proof.
+intros. induction H.
+- simpl. rewrite helper2. o_destruct; rewrite H.
+  all: constructor; rewrite helper; constructor.
+- simpl. rewrite o_Success. rewrite helper. constructor. constructor.
+  auto.
+- simpl. rewrite o_Failure. rewrite helper. constructor. constructor.
+  auto.
+Qed.
+
+Definition seq_configurations (c1 : Contract) (l0 l1 : list Contract) := 
+ (repeat (Failure::l1) (length l1))++[map (fun c => c _;_ c1) l0].
+
+Lemma plus_fold_flatten : forall c , plus_fold (flatten c) =R= c.
+Proof.
+induction c;intros;simpl;auto_rwd.
+rewrite c_eq_iff. setoid_rewrite plus_fold_app.
+rewrite <- c_eq_iff. rewrite IHc1.
+now rewrite IHc2.
+Qed.
+
+
+Lemma plus_fold_derive_flatten : forall (l : list Contract) (e : EventType), (plus_fold l) / e =R= plus_fold (flat_map (fun c => (flatten (c/e))) l).
+Proof.
+induction l;intros.
+- now simpl.
+- simpl. rewrite c_eq_iff. setoid_rewrite plus_fold_app.
+  rewrite <- c_eq_iff. rewrite IHl. now rewrite plus_fold_flatten.
+Qed.
+
+Lemma in_seq_configurations : forall c0 c1 l l0 l1, Flat_Seq_Derivative c0 c1 l -> AllDerivatives c0 l0
+-> AllDerivatives c1 l1 -> In_mod_R (plus_fold l) (n_prod (seq_configurations c1 l0 l1)).
+Proof.
+intros. unfold seq_configurations. induction H.
+- 
+-
+Lemma All_Derivatives_Seq : forall c0 c1 l l0 l1, Flat_Seq_Derivative c0 c1 l -> AllDerivatives c0 l0
+-> AllDerivatives c1 l1 -> AllDerivatives (plus_fold l) (n_prod (seq_configurations c1 l0 l1)).
+Proof.
+cofix IH.
+intros. econstructor.
+- intros. eapply AD_sub. symmetry. apply plus_fold_derive_flatten.
+  eapply IH;eauto. apply Flat_Seq_Derivative_closed; eauto.
+- unfold seq_configurations.
+
+
+
+
+  * auto.
+  * 
+ apply constructor.
+- intros. rewrite plus_fold_derive_flatten. eapply IH.
+  * eapply Flat_Seq_Derivative_closed. unfold seq_configurations.
+
+
+Ltac in_forall HF HIn := rewrite Forall_forall in HF; apply HF in HIn;destruct_ctx;subst.
+
+Lemma flatten_seq_derive_FSD : forall c0 c1 c_der s l, Flat_Seq_Derivative c0 c1 s (length s) l -> 
+ In c_der (flatten ((c0 _;_ c1) // s)) <-> ((exists c', c' =R= c_der /\ In c' l) \/ c_der =R= Failure).
+Proof. 
+intros. remember (length s). induction H.
+- simpl. symmetry in Heqn. apply length_zero_iff_nil in Heqn. subst. destruct (flatten_seq_derive_shape [] c0 c1). destruct H. split;intros.
+  * rewrite H in H1. simpl in H1. destruct H1.
+    ** subst. simpl. left. exists (c0 _;_ c1). split;auto.
+    ** in_forall H0 H1. simpl. destruct (o_or x0). 
+      *** rewrite H1. left. exists (c0 _;_ c1). split. split;auto.
+
+
+
+
+(**********************************)
+
+Lemma AllDerivatives_sub : forall c0 c1 l, c0 =R= c1 -> AllDerivatives c0 l -> AllDerivatives c1 l.
+Proof.
+cofix IH.
+intros. constructor. intros; simpl.
+- inversion H. eapply IH. inversion H. eauto. inversion H0. eauto.
+- inversion H0. destruct_ctx. subst. exists x. split;auto. now rewrite H2.
+Qed.
+
+Lemma AllDerivatives_sub_iff : forall c0 c1 l, c0 =R= c1 -> AllDerivatives c0 l <-> AllDerivatives c1 l.
+Proof.
+intros. split;eauto using AllDerivatives_sub. apply AllDerivatives_sub.
+now symmetry.
+Qed.
+
+Lemma plus_fold_plus : forall c0 c1, plus_fold [c0;c1] =R= c0 _+_ c1.
+Proof. c_eq_tac. Qed.
+
+Hint Resolve plus_fold_plus : coDB.
+
+(*
+Lemma AllDerivatives_Plus : forall (c0 c1 : Contract)(l0 l1 : list Contract), AllDerivatives c0 l0 -> AllDerivatives c1 l1 -> 
+ AllDerivatives (c0 _+_ c1) (n_prod [l0;l1]).
+Proof.
+cofix IH. intros. eapply AllDerivatives_sub. eapply plus_fold_plus. eapply AllDerivatives_Flatten_iff.
+eauto with coDB.
+Qed.
+Hint Resolve AllDerivatives_Plus : coDB.*)
+
+Lemma AllDerivatives_plus_plus_fold : forall (c0 c1 : Contract)(l : list Contract), AllDerivatives (c0 _+_ c1) l -> 
+ AllDerivatives (plus_fold [c0;c1] ) l.
+Proof. c_eq_tac. auto_rwd. inversion H. apply AllDerivatives_sub with(c0:= c0/e _+_ c1/e);
+       simpl in H0. auto_rwd. auto. inversion H. destruct_ctx.
+       exists x. auto_rwd.
+Qed.
+
+Lemma AllDerivatives_plus_fold_plus : forall (c0 c1 : Contract)(l : list Contract), 
+ AllDerivatives (plus_fold [c0;c1] ) l -> AllDerivatives (c0 _+_ c1) l .
+Proof.
+c_eq_tac. inversion H. simpl in H0.  apply AllDerivatives_sub with(c0:= c0/e _+_ (c1/e _+_ Failure));
+simpl. auto_rwd. auto. inversion H. destruct_ctx. exists x. simpl in H1.
+split;auto. now autorewrite with coDB in H1.
+Qed.
+
+(*coinductive definition can't handle rewriting as it violates constrctur guardedness*)
+Lemma AllDerivatives_plus_fold_iff : forall (c0 c1 : Contract)(l : list Contract), 
+ AllDerivatives (plus_fold [c0;c1] ) l <-> AllDerivatives (c0 _+_ c1) l.
+Proof. split;auto using AllDerivatives_plus_plus_fold,AllDerivatives_plus_fold_plus.
+Qed.
+
+
+Lemma AllDerivatives_comm : forall c0 c1 l, AllDerivatives (c0 _+_ c1) l -> AllDerivatives (c1 _+_ c0) l.
+Proof. c_eq_tac. inversion H;eauto. inversion H. destruct_ctx.
+       exists x. split;auto. rewrite H1. auto with coDB.
+Qed.
+
+Hint Immediate AllDerivatives_comm : coDB.
+
+
+Hint Resolve in_eq in_cons : core.
+
+Lemma AllDerivatives_Failure_seq : forall c, AllDerivatives (Failure _;_ c) ([Failure]).
+Proof.
+cofix IH.
+intros. constructor.
+- intros;simpl. rewrite o_Failure. eapply AllDerivatives_sub.  repeat rewrite c_eq_Failure_seq. 
+ symmetry. eapply c_eq_idempotent. auto with dpDB.
+- exists Failure. split;auto with dpDB. now rewrite c_eq_Failure_seq.
+Qed.
+
+Definition failure_seq_list l := map (fun l => Failure::l) (repeat l (length l)).
+
+Lemma AllDerivatives_nil : forall c, AllDerivatives c [] -> False.
+Proof.
+intros. inversion H. destruct_ctx. simpl in H4. contradiction.
+Qed.
+
+Search ((o _)/_).
+Locate o_derive.
+
+Ltac closure_sub c := apply AllDerivatives_sub with (c0:=c).
+
+Lemma AllDerivatives_o_seq : forall (l1 : list Contract)(c0 c1 : Contract),  AllDerivatives c1 l1 -> AllDerivatives ((o c0) _;_ c1) (Failure::l1).
+Proof.
+induction l1;intros. apply AllDerivatives_nil in H. contradiction. 
+constructor;intros.
+- simpl. autorewrite with icDB. closure_sub (o c0 _;_ c1 / e);auto_rwd.
+Admitted.
+(*
+  apply IH. Guarded. Guarded.   inversion H. eauto.  
+
+
+cofix IH.
+intros. constructor;intros.
+- destruct l1. apply AllDerivatives_nil in H. contradiction. simpl.
+  autorewrite with icDB. closure_sub (o c0 _;_ c1 / e);auto_rwd.
+  apply IH. Guarded. Guarded.   inversion H. eauto.  
+- destruct (o_or c0); destruct H0;rewrite H0.
+  * inversion H. destruct_ctx. exists x.
+    split;auto_rwd. auto.
+  * exists Failure. split;auto_rwd. auto.
+Qed.*)
+
+Lemma AllDerivatives_Seq : forall (c0 c1 : Contract)(l0 l1 : list Contract), AllDerivatives c0 l0 -> AllDerivatives c1 l1 -> AllDerivatives (c0 _;_ c1) (l0 ++l1).
+Proof.
+cofix IH.
+intros. constructor.
+- intros;simpl.
+
+ apply AllDerivatives_comm. unfold seq_closure. rewrite concat_n_prod.
+
+Lemma AllDerivatives_Seq : forall (c0 c1 : Contract)(l0 l1 : list Contract), AllDerivatives c0 l0 -> AllDerivatives c1 l1 -> AllDerivatives (c0 _;_ c1) (seq_closure c1 l0 l1).
+Proof. 
+cofix IH.
+intros. constructor.
+- intros. simpl. constructor. intros. simpl. cofix IH_plus. unfold seq_closure. rewrite concat_n_prod. 
+apply AllDerivatives_Plus.
+  * cofix IH_plus. constructor.
+    ** intros. simpl.
+
+ 
+
+
+Definition plus_combine (l0 l1 : list Contract) := map (fun p => (fst p) _+_ (snd p)) (combine l0 l1).
+
+
+
+
+
+(****************Code below hasn't been cleaned up**********************************************************)
+
+
+(*
+Fixpoint In_mod_ACI (c : Contract) (l : list Contract) :=
+match l with
+| [] => False
+| c' ::l' => c' =ACI= c \/ In_mod_ACI c l'
+end.
+
+Lemma In_mod_ACI_i_In : forall (c : Contract) (l : list Contract), In_mod_ACI c l -> exists c', In c' l /\ c' =ACI= c.
+Proof.
+intros c l. generalize dependent c. induction l;intros.
+- simpl in H. inversion H.
+- simpl in H. destruct H.
+  * exists a. split;auto using in_eq.
+  * apply IHl in H. destruct H. exists x. destruct H. split;auto using in_cons.
+Qed.
+
+Lemma In_i_In_mod_ACI : forall (c : Contract) (l : list Contract), (exists c', In c' l /\ c' =ACI= c) -> In_mod_ACI c l.
+Proof.
+intros. generalize dependent c. induction l;intros.
+- destruct H. destruct H. simpl in H. inversion H.
+- simpl. destruct H. destruct H. simpl in H. inversion H.
+  * subst. now left.
+  * right. apply IHl. exists x;split;auto.
+Qed.
+
+Theorem In_mod_ACI_iff_In : forall (c : Contract) (l : list Contract), In_mod_ACI c l <-> exists c', In c' l /\ c' =ACI= c.
+Proof.
+split; auto using In_i_In_mod_ACI.
+intros. now apply In_mod_ACI_i_In.
+Qed.
+
+Theorem In_mod_ACI_cons : forall (c c' : Contract) (l : list Contract), In_mod_ACI c (c'::l) <-> c' =ACI= c \/ In_mod_ACI c l.
+Proof.
+split;intros.
+- rewrite In_mod_ACI_iff_In in H. destruct_ctx. induction H.
+  * subst. now left.
+  * right. rewrite In_mod_ACI_iff_In. exists x. split;auto.
+- destruct H.
+  * rewrite In_mod_ACI_iff_In. exists c'. split;auto using in_eq.
+  * rewrite In_mod_ACI_iff_In in *. destruct_ctx. exists x.
+    split;auto using in_cons,in_eq.
+Qed. *)
+
+Lemma lift_bmatches : forall c0 c1, (forall s, nu (c0//s) = nu (c1//s)) -> c0 =R= c1.
+Proof.
+intros. rewrite c_eq_iff. intros. specialize H with s. repeat rewrite Matches_Comp_iff_matchesb.
+rewrite H. reflexivity.
+Qed.
+
+Lemma c_eq_idempotent : forall c, c _+_ c =R= c.
+Proof.
+cofix IH.
+intros. constructor. intros. simpl. auto. simpl. btauto.
+Qed.
+
+
+Ltac nu_solve := simpl ; try btauto.
+
+
+
+Ltac derive_plus_tac H := rewrite derive_plus in H; simpl in H; apply in_app_or in H; destruct H.
+
+(*Reduce all failure cases to Failure*)
+Theorem in_flatten_seq_i_Failure_derive : forall s c1 c_der, In c_der (flatten ((Failure _;_ c1) // s)) -> 
+c_der =b= Failure.
+Proof.
+induction s;intros.
+- simpl in H. destruct H;try contradiction. inversion H. subst.
+  auto_rwd.
+- auto_rwd. simpl in H. auto_rwd_in H. simpl in H. apply in_app_or in H.
+  destruct H. apply IHs with (s:=s0) in H. rewrite H. auto_rwd.
+  apply IHs with (s:=s0) in H. rewrite H. auto_rwd.
+Qed.
+
+Theorem Failure_derive_i_in_flatten_seq : forall s c1, exists c_der, c_der =b= Failure /\ 
+ (In c_der (flatten ((Failure _;_ c1) // s))).
+Proof.
+induction s;intros.
+- exists (Failure _;_ c1). simpl. split;autoM.
+- simpl. auto_rwd. simpl. specialize IHs with c1 as IHs'. destruct_ctx. exists x.
+  split;autoM. rewrite in_app_iff.  now left. 
+Qed.
+
+Definition bool_incl_lists (l0 l1 : list Contract) := forall c, In c l0 -> exists c', In c' l1 /\ c' =b= c.
+
+Definition bool_equiv_lists (l0 l1 : list Contract) := bool_incl_lists l0 l1 /\ bool_incl_lists l1 l0.
+
+
+Lemma test : forall s c, bool_equiv_lists (flatten ((Failure _;_ c) // s)) [Failure].
+Proof.
+intros. unfold bool_equiv_lists,bool_incl_lists. split.
+- intros. pose proof Failure_derive_i_in_flatten_seq s c. destruct_ctx.
+  exists x.
+Admitted.
+
+Theorem in_flatten_seq_o_derive : forall s c0 c1 c_der, In c_der (flatten (((o c0) _;_ c1) // s)) -> 
+c_der =b= Failure \/ c_der =b= (o c0) _;_ c1//s. 
+Proof.
+induction s;intros.
+- simpl in H. destruct H;try contradiction. inversion H. destruct (o_or c0).
+  * rewrite H1. right. autoM.
+  * rewrite H1. left. autoM. 
+- simpl in H. auto_rwd_in H. simpl in H. apply in_app_or in H. destruct H.
+  * rewrite o_derive in H. eauto using in_flatten_seq_i_Failure_derive.
+  * rewrite o_idempotent in H. apply IHs in H. destruct H.
+    ** now left.
+    ** right. now simpl.
+Qed.
+
+
+Theorem in_flatten_seq_derive : forall s c0 c1 c_der, In c_der (flatten ((c0 _;_ c1) // s)) -> 
+c_der =b= Failure \/ (exists l0 l1 , s = l0++l1 /\ c_der =b= (o (c0 // l0)) _;_ c1 // l1) \/ (c_der =b= c0//s _;_ c1).
+Proof.
+induction s;intros.
+- simpl in H. destruct H; try contradiction. subst. right. right. auto.
+- simpl in H. auto_rwd_in H. simpl in H. apply in_app_or in H.
+  destruct H.
+  * apply IHs in H. destruct H.
+    ** now left.
+    ** destruct H. 
+      *** destruct_ctx. subst. right. left. exists (a::x). exists x0.
+          split;auto.
+      *** right. right. auto.
+  * apply in_flatten_seq_o_derive in H. destruct H;auto. 
+    right. left. exists []. exists (a::s). split;auto.
+Qed.
+
+Definition seq_derive_cases (c0 c1 :Contract) := [c0 ; c1].
+Lemma test2 : forall s c0 c1, bool_equiv_lists (flatten ((c0 _;_ c1) // s)) (seq_derive_cases c0 c1).
+Proof. Admitted.
+Definition plus_fold (l : list Contract) := Failure.
+Lemma bool_equiv_AllDerivatives : forall (pl0 pl1 l : list Contract) (c : Contract), bool_equiv_lists pl0 pl1 ->
+ AllDerivatives (plus_fold pl0) l <-> AllDerivatives (plus_fold pl1) l.
+
+Lemma AllDerivatives_Seq : forall (c0 c1 : Contract)(l0 l1 : list Contract), AllDerivatives c0 l0 -> AllDerivatives c1 l1 -> 
+ AllDerivatives (c0 _;_ c1) ((map (fun c => c _;_ c1) l0) ++ ) l1).
+
+Theorem in_flatten_seq_derive : forall s c0 c1 c_der0 c_der1, In (c_der0 _;_ c_der1) (flatten ((c0 _;_ c1) // s)) <-> 
+(c_der0 _;_ c_der1 = c0 // s _;_ c1) \/ ( s<> [] /\ (c_der0 = Success \/ c_der0 = Failure) /\ exists n_lo n_hi, c_der1 = c1//(firstn n_hi (skipn n_lo s))).
+Proof.
+intro. 
+induction s;intros;simpl.
+- split;intros. destruct H;try contradiction. inversion H. subst. now left.
+  destruct H. inversion H. now left. destruct_ctx. contradiction.
+- split;intros.
+  * rewrite derive_plus in H. simpl in H. apply in_app_or in H. destruct H.
+    ** apply IHs in H. destruct H.
+      *** now left.
+      *** destruct_ctx. destruct H0.
+        **** subst. right. split.  intro H2.  discriminate. split. now left. 
+             exists (S x). exists x0. now simpl.
+        **** subst. right. split. intro H2. discriminate. split. now right.
+             exists (S x). exists x0. now simpl.
+    ** apply IHs in H. destruct H.
+      *** inversion H. subst. right. split. intro H2. discriminate.
+          split. destruct (o_or c0). rewrite H0. 
+          destruct s. simpl. now left. simpl. rewrite Failure_trace_derive.
+          now right. rewrite H0. rewrite Failure_trace_derive. now right.
+          exists 0. exists 1. simpl. auto.
+      *** destruct_ctx. subst. destruct H0.
+        **** rewrite H0. right. split;auto. intro H2. discriminate.
+             split. now left. exists 0. exists x0.
+ Check trace_derive_failure. rewrite  r simpl; left.
+ intuition;try contradiction. auto.
+ destruct H;subst.
+  exists 1. now simpl. split. destruct H. inversion H. subst.
+  destruct (o_or c0). rewrite H0. right. now left. rewrite H0. right. right. auto.
+  inversion H. inversion H. inversion H0. subst. exists 0. now simpl.
+  inversion H0. destruct_ctx. destruct H. destruct x.
+  * simpl in H0. subst. intuition. auto.
+ subst. destruct H;subst. simpl. now right. susbt. 
+ rewrite H.
+ rewrite Heqt in *. simpl in H. destruct H;try contradiction. inversion H.
+  now left. destruct H. rewrite Heqt. simpl. auto. now left.
+  destruct H. subst.  rewrite H.
+
+
+
+Theorem in_flatten_seq_Failure_derive : forall s c1 c_der0 c_der1, In (c_der0 _;_ c_der1) (flatten ((Failure _;_ c1) // s)) <-> 
+c_der0 = Failure /\ exists n_low n_high, c_der1 = c1//(skipn n_low (firstn n_high s)).
+Proof.
+induction s;intros.
+- split;intros;simpl in *. destruct H;try contradiction. inversion H. subst.
+  split;auto. exists 0. exists 0. now simpl. destruct_ctx.
+  rewrite firstn_nil in H0. rewrite skipn_nil in H0. subst. left; now simpl.
+- split;intros.
+  * simpl in H. derive_plus_tac H. 
+    ** apply IHs in H. destruct_ctx. subst. split;auto. exists (S x). now simpl.
+    ** apply IHs in H. destruct_ctx. subst. split;auto. exists (S x).
+
+Ltac derive_plus_tac H := rewrite derive_plus in H; simpl in H; apply in_app_or in H; destruct H.
+Theorem in_flatten_seq_o_derive : forall s e c0 c1 c_der0 c_der1, In (c_der0 _;_ c_der1) (flatten (((o c0) _;_ c1) // (e::s))) <-> 
+(c_der0 = Failure /\ exists n, c_der1 = c1//(firstn n s)) \/ (c_der0 = o c0 /\ exists n, c_der1 = c1//(e::(firstn n s))).
+Proof.
+induction s;intros.
+- split;intros;simpl. destruct H;try contradiction. inversion H. subst.
+  left.  split;autoC. exists 0. now simpl. destruct H;try contradiction. 
+  inversion H. subst. right. split;autoC. exists 1. now simpl.
+  destruct H. destruct_ctx. subst. left. simpl. rewrite firstn_nil.
+  rewrite o_derive. auto.  destruct_ctx. destruct x. simpl in H0. subst. subst. right.
+  rewrite o_idempotent. 
+  auto. simpl in H0. subst. right. left. rewrite o_idempotent. auto.
+- split;intros.
+  * simpl trace_derive in H. remember (a::s). simpl in H.
+    derive_plus_tac H. rewrite Heql in H. rewrite o_derive in H.
+    assert (HA : Failure = o Failure). { auto. } rewrite HA in H.
+    apply IHs in H. destruct H.
+    ** destruct_ctx. subst. left.
+ rewrite <- Heql in H. simpl in H. fold in H. derive_plus_tac H. 
+    ** simpl in IHs. rewrite o_derive in H. assert (HA : Failure = o Failure). { auto. }
+       rewrite HA in H. setoid_rewrite o_idempotent in IHs. 
+       rewrite o_idempotent in H. apply IHs in H. destruct H.
+      *** destruct_ctx. subst. left. split;auto. destruct H. derive_plus_tac H.
+      *** simpl in IHs. rewrite derive_plus in H. simpl in H. simpl in H.
+
+
+
+ left.
+  destruct (o_or c0); intuition. now exists 0. left. symmetry. destruct_ctx.
+  destruct (o_or c0). destruct H. subst. rewrite H1. rewrite skipn_nil. auto.
+  destruct H. contradiction. destruct H. subst. rewrite skipn_nil. auto.
+  destruct H. contradiction.
+- split;intros.
+  * rewrite derive_plus in H. simpl in H. apply in_app_or in H. destruct H.
+    ** rewrite o_derive in H. assert (HA: Failure = o Failure). auto.
+       rewrite HA in H. apply IHs in H. destruct_ctx. subst. split.
+      *** destruct H.
+        **** subst. right. split. intro H3. discriminate. auto.
+        **** destruct H. subst. right. split. intro H3. discriminate. auto.
+      *** destruct H. subst. exists (S x). auto. exists (S x). auto.
+    ** apply IHs in H. destruct_ctx. subst. destruct H.
+      *** split. subst. rewrite o_idempotent. now left. split.
+ 
+
+  subst. rewrite H1. left.
+  destruct H. subst.  inversion H. now left. destruct_ctx. contradiction.
+
+Theorem in_flatten_seq_derive : forall s c0 c1 c_der0 c_der1, In (c_der0 _;_ c_der1) (flatten ((c0 _;_ c1) // s)) <-> 
+(c_der0 _;_ c_der1 = c0 // s _;_ c1) \/ ( s<> [] /\ (c_der0 = Success \/ c_der0 = Failure) /\ exists n, c_der1 = c1//(skipn n s)).
+Proof.
+intro. 
+induction s;intros;simpl.
+- split;intros. destruct H;try contradiction. inversion H. subst. now left.
+  destruct H. inversion H. now left. destruct_ctx. contradiction.
+- split;intros.
+  * rewrite derive_plus in H. simpl in H. apply in_app_or in H. destruct H.
+    ** apply IHs in H. destruct H.
+      *** now left.
+      *** destruct_ctx. destruct H0.
+        **** subst. right. split.  intro H2.  discriminate. split. now left. 
+             exists (S x). now simpl.
+        **** subst. right. split. intro H2. discriminate. split. now right.
+             exists (S x). now simpl.
+    ** apply IHs in H. destruct H.
+      *** inversion H. subst. left. simpl; left.
+ intuition;try contradiction. auto.
+ destruct H;subst.
+  exists 1. now simpl. split. destruct H. inversion H. subst.
+  destruct (o_or c0). rewrite H0. right. now left. rewrite H0. right. right. auto.
+  inversion H. inversion H. inversion H0. subst. exists 0. now simpl.
+  inversion H0. destruct_ctx. destruct H. destruct x.
+  * simpl in H0. subst. intuition. auto.
+ subst. destruct H;subst. simpl. now right. susbt. 
+ rewrite H.
+ rewrite Heqt in *. simpl in H. destruct H;try contradiction. inversion H.
+  now left. destruct H. rewrite Heqt. simpl. auto. now left.
+  destruct H. subst.  rewrite H.
+
+
+c_der = (c0//s _;_ c1) \/ (s <> [] /\ exists n, c_der = Success _;_ (c1 // (skipn n s)) \/ c_der = Failure _;_ (c1 // (skipn n s))).
+Proof.
+induction s;intros.
+- simpl. split;intros. destruct H. now left. contradiction. destruct H. now left.
+  destruct_ctx. destruct H. auto.
+- split;intros.
+  * simpl in H. rewrite derive_plus in H. simpl in H.
+    apply in_app_or in H. destruct H.
+    ** apply IHs in H. destruct H.
+      *** left. now simpl.
+      *** right. split;auto. intro H3. discriminate. destruct_ctx.
+          destruct H0.
+        **** rewrite H0. exists (S x). simpl. now left.
+        **** rewrite H0. exists (S x). simpl. now right.
+    ** apply IHs in H. destruct H.
+      *** right. split. intro H3. discriminate. rewrite H.
+          destruct (o_or c0).
+        **** rewrite H0. exists ( left;simpl;auto. auto. subst. simpl. rewrite IHs.
+   split split;intros.
+  * inversion H;try contradiction. now left.
+  * destruct H. now left. destruct H. destruct H.
+    ** simpl in H.
+
+
+ destruct s. 
+      *** simpl in H. destruct H;try contradiction.
+          right. split. intro. discriminate. rewrite <- H. exists 0.
+          destruct (o_or c0);rewrite H0; auto || auto.
+      *** rewrite flatten_seq_trace_derive in H. rewrite in_flat_map in H.
+          destruct_ctx.
+        **** inversion
+
+
+
+
+ ((c0 // s) _;_ c1):: l /\
+ Forall (fun c => exists c' s, c = (o c') _;_ (c1//s)) l.
+
+
+Check firstn.
+Inductive Flat_Seq_Derivative : Contract -> Contract -> Trace -> nat -> list Contract -> Prop :=
+| FSD_Single c0 c1 s : Flat_Seq_Derivative c0 c1 s 0 [c0//s _;_ c1]
+| FSD_Cons c0 c1 s n l (H: Flat_Seq_Derivative c0 c1 s n l) : Flat_Seq_Derivative c0 c1 s (S n) (c1//(firstn (S n) s)::l).
+
+Ltac in_forall HF HIn := rewrite Forall_forall in HF; apply HF in HIn;destruct_ctx;subst.
+
+Lemma flatten_seq_derive_FSD : forall c0 c1 c_der s l, Flat_Seq_Derivative c0 c1 s (length s) l -> 
+ In c_der (flatten ((c0 _;_ c1) // s)) <-> ((exists c', c' =R= c_der /\ In c' l) \/ c_der =R= Failure).
+Proof. 
+intros. remember (length s). induction H.
+- simpl. symmetry in Heqn. apply length_zero_iff_nil in Heqn. subst. destruct (flatten_seq_derive_shape [] c0 c1). destruct H. split;intros.
+  * rewrite H in H1. simpl in H1. destruct H1.
+    ** subst. simpl. left. exists (c0 _;_ c1). split;auto.
+    ** in_forall H0 H1. simpl. destruct (o_or x0). 
+      *** rewrite H1. left. exists (c0 _;_ c1). split. split;auto.
+
+
+
+  * inversion H1. subst. rewrite H.  auto using in_eq. contradiction.
+  * rewrite H in H1. simpl in H1. destruct H1;auto.
+    rewrite Forall_forall in H0. apply H0 in H1. destruct_ctx. subst.
+    ** now left. 
+    rewrite Forall_forall in H1.
+
+Lemma FSD_max_length : forall c0 c1 c_der s l, n > length s ->  Flat_Seq_Derivative c0 c1 s n l ...
+
+Definition seq_closure_list (c0 c1 : Contract) (l0 l1 : list Contract) := 
+ let first_elements := map (fun c => c _;_ c1) l0 in
+ let mid_success_elems := map (fun c => Success _;_ c) l1 in
+ let mid_failure_elems := map (fun c => Failure _;_ c) l1 in
+ 
+
+
+
+
+(*Lemma Trace_Derive_seq_tail : forall  l e s c0 c1 c', flatten ((c0 _;_ c1) // s) = e::l ->
+In c' l -> exists c'' n, Trace_Derive c1 (firstn n s) c'' /\ (c' = Success _;_ c'' \/ c' = Failure _;_ c'').
+Proof.
+induction l;intros.
+- simpl in H0. inversion H0.
+- simpl in H0. inversion H0.
+  * rewrite derive_plus in H. simpl in H.
+  destruct (flatten_non_empty ((c0 / a _;_ c1) // s)).
+  destruct_ctx. rewrite H0 in H. simpl in H. apply in_app_or in H.
+  destruct H.
+  *
+
+  destruct (flatten_non_empty ((c0 _;_ c1) // (a :: s))).
+Trace_Derive (c0 _;_ c1) s c_der -> In_mod_ACI c_der ???
+
+
+
+Definition decompose_seq_aux (c0 c1 : Contract) (s : Trace) := 
+match s with
+| [] => if nu c0 then
+ (trace_derive c0 s) _;_ c1 _+_ 
+
+
+Lemma Trace_Derive_seq : forall (c0 c1 c_der : Contract)(s : Trace), Trace_Derive (c0 _;_ c1) s c_der ->
+ c_der =ACI= *)
+
+Lemma plus_prod_length : forall (l0 l1 : list Contract), length (plus_prod l0 l1) = length l0 * length l1.
+Proof.
+intros. unfold plus_prod. rewrite map_length. now rewrite prod_length.
+Qed.
+
+Hint Resolve AllDerivatives_Plus  : dpDB.
+
+Lemma exists_finite_closure : forall (c : Contract), exists (l : list Contract), AllDerivatives c l /\ length l = max_derivative_count c.
+Proof.
+induction c;intros.
+- exists [Success;Failure]. split;auto with dpDB. 
+- exists [Failure]. split;auto with dpDB.
+- exists [Event e;Success;Failure]. split;auto with dpDB.
+- destruct_ctx. exists (plus_prod x0 x). split;simpl; auto with dpDB.
+  rewrite plus_prod_length. rewrite H2. now rewrite H0.
+-
+  rewrite prod_length.
+  simpl.
+
+Definition simple_derivative_closure (c : Contract) := simple_n_derivative_closure c (max_derivative_count c).
+
+
+Eval compute in flat_map (nth_derivatives Failure) (seq 0 1).
+Lemma simple_derivative_closure_spec_helper : forall (n:nat)(c : Contract)(s:Trace), length s <n -> 
+In (trace_derive c s) (flat_map (nth_derivatives c) (seq 0 n)).
+Proof.
+induction n;intros.
+- simpl. destruct s;simpl in H; inversion H.
+- rewrite in_flat_map. exists (length s). split; auto using nth_derivatives_spec.
+  rewrite in_seq. simpl.  unfold lt. split; auto.
+    transitivity (length s);lia.
+Qed.
+
+
+Lemma in_simple_derivative_closure : forall (c : Contract)(s : Trace), length s < max_derivative_count c ->
+ In (trace_derive c s) (simple_derivative_closure c).
+Proof.
+intros. unfold simple_derivative_closure. now apply simple_derivative_closure_spec_helper.
+Qed.
+
+Lemma in_simple_derivative_closure_failure_success : In Failure (simple_derivative_closure Success).
+Proof. unfold simple_derivative_closure. rewrite in_flat_map. exists 1.
+rewrite in_seq.
+split;auto. rewrite <- (trace_derive_failure [Transfer]). apply nth_derivatives_spec.
+Qed.
+
+Lemma in_simple_derivative_closure_success_event : forall (e : EventType), In Success (simple_derivative_closure (Event e)).
+Proof.
+intros.
+unfold simple_derivative_closure. rewrite in_flat_map. exists 1.
+rewrite in_seq.
+split;simpl;auto. assert (HA: Success = (trace_derive (Event e) [e])). { simpl. now eq_event_destruct. }
+rewrite HA. apply nth_derivatives_spec.
+Qed.
+
+Hint Unfold simple_derivative_closure : core.
+
+(*
+Lemma in_simple_derivative_closure_trans : forall (c0 c1 c2 : Contract), In c0 (simple_derivative_closure c1) ->
+In c1 (simple_derivative_closure c2) -> In c0 (simple_derivative_closure c2).
+Proof.
+intros. unfold simple_derivative_closure in *. rewrite in_flat_map in *.
+destruct H. destruct H0. exists (x+x0). split.
+- destruct H. destruct H0. rewrite in_seq in *. split;simpl in *. lia.*)
+
+Lemma in_simple_derivative_closure_failure_event : forall (e : EventType), In Failure (simple_derivative_closure (Event e)).
+Proof.
+intros.
+ unfold simple_derivative_closure. rewrite in_flat_map. exists 1.
+ split;simpl;auto. destruct ((exists_disimilar_event e)). 
+ assert (HA: Failure = trace_derive (Event e) [x]). { simpl. now eq_event_destruct. }
+ rewrite HA. apply nth_derivatives_spec.
+Qed.
+
+Print In.
+
+ 
+
+(*
+Lemma In_mod_ACI_iff : forall (f : Contract -> Contract) 
+         (l : list Contract) (y : Contract), ACI_preserving f ->
+       In_mod_ACI y (map f l) <->
+       (exists x : Contract, f x =ACI= y /\ In_mod_ACI x l).
+Proof.
+split;intros.
+- rewrite In_mod_ACI_iff_In in H0. destruct H0. destruct H0.
+  rewrite in_map_iff in H0. destruct H0. destruct H0. exists x0. 
+  rewrite H0. split;auto. rewrite In_mod_ACI_iff_In. exists x0. split;auto.
+- destruct H0. destruct H0. rewrite In_mod_ACI_iff_In. 
+  rewrite In_mod_ACI_iff_In in H1. destruct H1. exists (f x0). split.
+  * rewrite in_map_iff. exists x0. destruct H1. split ;auto.
+  * destruct H1. inversion H0.
+    ** rewrite H4. auto. subst. unfold ACI_preserving in H. auto.
+    **
+ f_equal. symmetry in H1. auto.
+  rewrite In_mod_ACI_iff_In in H0. destruct H0. destruct H0. exists  exists (f x).
+  split;auto. rewrite in_map_iff. 
+    split;auto. exists x.
+   rewrite in_map_iff in H. destruct H. destruct H. exists x. split;auto.
+  rewrite In_mod_ACI_iff_In. exists x. split;auto.
+- destruct H. destruct H. rewrite in_map_iff. exists x.
+intros. split;intros.*)
+
+Ltac In_mod_destruct H := rewrite In_mod_ACI_iff_In in H; destruct H; destruct H;
+rewrite in_map_iff in H; destruct H; destruct H.
+Definition simple_n_derivative_closure (c : Contract) (n:nat) := flat_map (nth_derivatives c) (seq 0 n).
+Definition plus_combine (l0 l1 : list Contract) := map (fun p => (fst p) _+_ (snd p)) (combine l0 l1).
+Lemma simple_derivative_closure_plus : forall c0 c1, simple_derivative_closure (c0 _+_ c1) =
+plus_combine (simple_n_derivative_closure c0 (max_derivative_count (c0 _+_ c1))) 
+             (simple_n_derivative_closure c1 (max_derivative_count (c0 _+_ c1))).
+Proof. Admitted.
+
+Lemma derivative_closure_in_list_prod : forall c0 c1 c_der,
+  (forall s, In_mod_ACI (trace_derive c0 s) (simple_derivative_closure c0)) -> 
+  (forall s, In_mod_ACI (trace_derive c1 s) (simple_derivative_closure c1)) -> 
+  In_mod_ACI c_der (map (fun p => (fst p) _+_ (snd p))(list_prod (simple_derivative_closure c0) (simple_derivative_closure c1)))
+ -> In_mod_ACI c_der (simple_derivative_closure (c0 _+_ c1)).
+Proof. 
+intros. rewrite simple_derivative_closure_plus. rewrite In_mod_ACI_iff_In.
+In_mod_destruct H1. destruct x0.
+rewrite in_prod_iff in H3. destruct H3.
+subst. simpl in H2. exists (c _+_ c2). subst. simpl in H2. split;auto.
+unfold simple_derivative_closure. simpl.
+-
+
+ rewrite In_mod_ACI_iff_In in H1. destruct H1. destruct H1.
+rewrite in_map_iff in H1. destruct H1. destruct H1.
+rewrite In_mod_ACI_iff_In.
+(*Lemma derivative_closure_in_list_prod : forall c0 c1 c_der, In c_der (simple_derivative_closure (c0 _+_ c1)) 
+-> In_mod_ACI c_der (map (fun p => (fst p) _+_ (snd p))(list_prod (simple_derivative_closure c0) (simple_derivative_closure c1))).
+Proof.
+intros. unfold simple_derivative_closure in H. rewrite in_flat_map in H.
+destruct H. destruct H. rewrite 
+
+Lemma simple_derivative_closure_plus : forall (c0 c1 : Contract)(s : Trace),
+ (forall s, exists c0', trace_derive c0 s =ACI= c0' /\ In c0' (simple_derivative_closure c0)) ->
+ (forall s, exists c1', trace_derive c1 s =ACI= c1' /\ In c1' (simple_derivative_closure c1)) ->
+ exists c', trace_derive (c0 _+_ c1) s =ACI= c' /\ 
+ In c' (map (fun p => (fst p) _+_ (snd p))(list_prod (simple_derivative_closure c0) (simple_derivative_closure c1))).
+Proof.
+intros.
+Admitted.*)
+(* unfold simple_derivative_closure in H1. rewrite in_flat_map in H1.
+destruct H1. destruct H1. unfold nth_derivatives in H2. rewrite in_map_iff in H2.
+destruct H2. destruct H2. rewrite trace_derive_plus in H2.
+rewrite in_map_iff. specialize H with x0. specialize H0 with x0.
+destruct H. destruct H. destruct H0. destruct H0. exists (x1, x2).
+split. injection H2. exists (trace_derive c0 x0, trace_derive c1 x0).
+split.
+- now simpl.
+- rewrite in_prod_iff. split. simpl in H. rewrite in_seq in H. destruct H.
+simpl in H2. pose proof (n_length_traces_length x). rewrite Forall_forall in H3. 
+apply H3 in H1. apply in_simple_derivative_closure. rewrite H1. Search (?a < ?b * _).
+assert (HA: x = x * 1). { lia. } rewrite HA in H2. SearchRewrite (1 * _).
+ lia. subst. unfold incl. intr*)
+
+(*To show P for derivative_closure of c0 _+_ c1, it suffices to show it for cartesian product of c0' and c1's closure*)
+
+
+(*Contracts from all ACI equivalence classes are present in the simple derivative closure *)
+Lemma simple_derivative_closure_spec : forall (c : Contract) (s : Trace), 
+In_mod_ACI (trace_derive c s) (simple_derivative_closure c).
+Proof.
+induction c;intros.
+- rewrite In_mod_ACI_iff_In. destruct (trace_derive_success s).
+  * exists Success. rewrite H. saia. 
+  * exists Failure. rewrite H. split;auto using in_simple_derivative_closure_failure_success.
+- rewrite In_mod_ACI_iff_In. exists Failure. saia.
+- rewrite In_mod_ACI_iff_In. destruct (trace_derive_event s e).
+  * exists (Event e). rewrite H. saia.
+  * destruct H.
+    ** exists Success. rewrite H. split; auto using in_simple_derivative_closure_success_event. 
+    ** exists Failure. rewrite H. split;auto using in_simple_derivative_closure_failure_event.
+- apply derivative_closure_in_list_prod;auto.
+  specialize IHc1 with s. specialize IHc2 with s. rewrite In_mod_ACI_iff_In in *.
+  destruct IHc1. destruct IHc2. exists (x _+_ x0). split.
+  * rewrite in_map_iff. exists (x, x0). split;auto.
+    destruct H. destruct H0.
+    apply in_prod;auto.
+  * rewrite trace_derive_plus. destruct H. destruct H0.
+    rewrite H1. now rewrite H2.
+-
+ Admitted. 
+
+
+
+(*All derivatives of c can be found with traces of size max_derivative_count c or less *)
+(*Remember rewrite c0 _;_ c1 / e to using the o-notation*)
+Theorem finite_distinct_derivatives : forall (c : Contract)(s : Trace), exists s', 
+ length s' < max_derivative_count c /\ (trace_derive c s) =ACI= (trace_derive c s').
+Proof with (simpl;intuition || auto). 
+induction c;intros.
+- simpl. destruct s;simpl.
+  * exists []. saia. 
+  * exists [Transfer]. saia. 
+- simpl. exists []. saia. 
+- simpl. destruct s eqn:Heqn.
+  * exists []. saia.
+  * simpl. eq_event_destruct.
+    ** destruct (trace_derive_success t);rewrite H.
+      *** exists [e]. simpl. eq_event_destruct; saia. 
+      *** destruct (exists_disimilar_event e). exists [x]. simpl.
+          eq_event_destruct. contradiction. saia.
+    ** destruct (exists_disimilar_event e). exists [x]. simpl.
+          eq_event_destruct. contradiction. saia.
+- simpl. setoid_rewrite trace_derive_plus. induction s.
+  * exists []. simpl. split;auto.
+    rewrite (mult_n_O 0) at 1. auto using PeanoNat.Nat.mul_lt_mono, max_derivative_count_non_zero.
+  *
+    ** 
+
+ exists [].
+-
+    ** exists [e]. saia.
+  simpl. intuition || auto.
+ assert (HA : exists 
+
+
+
+
+
+
+
+(*Drawback, contains duplicates*)
+Definition derivative_closure_once (l_pair : (list Contract) * (list Contract)) :=
+ let (internal_nodes,leafs) := l_pair in
+ (internal_nodes++leafs,flat_map (fun c => map (fun e => c/e) alphabet) leafs).
+
+
+
+(*include c in left list to represent value of (trace_derive c []) *)
+(*More effecient way to compute derivative closure than trivially iterating over all trace with trace_derive*)
+Definition approx_derivative_closure (n : nat) (c : Contract) :=
+ approx n derivative_closure_once ([c],[c]).
+
+Lemma trace_derive_in_derivative_closure_snd : forall (c : Contract) (s : Trace), In (trace_derive c s) (snd (approx_derivative_closure (length s) c)).
+Proof. Admitted.
+
+Lemma derivative_closure_snd_in_fst : forall n n' c c_der , In c_der (snd (approx_derivative_closure n c)) -> 
+                                                            n<n' -> In c_der (fst (approx_derivative_closure n' c)).
+Proof. Admitted.
+
+Definition derivative_closure (c : Contract) : list Contract := fst (approx_derivative_closure (max_derivative_count c) c).
+
+Lemma simple_derivative_closure_i_derivative_closure : forall c,incl (simple_derivative_closure c) (derivative_closure c).
+Proof. Admitted.
+
+Lemma derivative_closure_i_simple_derivative_closure : forall c,incl (derivative_closure c) (simple_derivative_closure c).
+Proof. Admitted.
+
+Lemma derivative_closure_spec : forall (c : Contract), contains_all_derivatives_of c (derivative_closure c).
+Proof. Admitted.
+
+
+(*********************************************Extend to pairs of contracts***************************)
+Fixpoint trace_p_derive (p: Contract * Contract) (s : Trace) :=
+match s with
+| [] => p
+| e::s' => trace_p_derive (fst p / e, snd p /e) s'
+end.
+
+
+Definition p_derivative_closure_once (l_pair : (list (Contract*Contract)) * (list (Contract * Contract))) :=
+ let (internal_nodes,leafs) := l_pair in
+ (internal_nodes++leafs,flat_map (fun p => map (fun e => ((fst p) / e,(snd p) / e)) alphabet) leafs).
+
+Definition approx_p_derivative_closure (n : nat) (p : (Contract * Contract)) :=
+ approx n p_derivative_closure_once ([p],[p]).
+
+Lemma trace_derive_in_p_derivative_closure_snd : forall (c0 c1: Contract) (s : Trace), In (trace_p_derive (c0,c1) s) (snd (approx_p_derivative_closure (length s) (c0,c1))).
+Proof. Admitted.
+
+Lemma p_derivative_closure_snd_in_fst : forall n n' p p_der , In p_der (snd (approx_p_derivative_closure n p)) -> 
+                                                            n<n' -> In p_der (fst (approx_p_derivative_closure n' p)).
+Proof. Admitted.
+
+Definition max_p_derivative_count (p : Contract * Contract) := (max_derivative_count (fst p)) * (max_derivative_count (snd p)).
+
+Definition all_p_derivatives (p : Contract * Contract) : list (Contract * Contract) := fst (approx_p_derivative_closure (max_p_derivative_count p) p).
+
+Lemma all_p_derivatives_spec : forall (c0 c1 : Contract)(s : Trace), In (trace_p_derive (c0,c1) s) (all_p_derivatives (c0,c1)).
+Proof. Admitted.
+
+
+(*Show lemma that all derivatives are in derivative_closure*)
+Lemma derivative_closure_is_bisimulation : forall (c0 c1 : Contract), 
+ Forall (fun (p : Contract * Contract) => nu (fst p) = nu (snd p)) (all_p_derivatives (c0,c1)) -> bisimulation (fun x y => (In (x,y) (all_p_derivatives (c0,c1)))).
+Proof. Admitted.
+
+Definition decide_contract_equivalence (c0 c1 : Contract) := 
+ forallb (fun (p : Contract * Contract) => eqb (nu (fst p)) (nu (snd p))) (all_p_derivatives (c0,c1)).
+
+
+Lemma Bisimilarity_reflect : forall (c0 c1 : Contract), reflect (Bisimilarity c0 c1) (decide_contract_equivalence c0 c1).
+Proof. Admitted.
+
+
+
+
+
+
+
+
+
+
+
+
+
+
+
+
+
+
+
+
+
+
+
+
+
+
+
+
+
+
+
+
+(*
+Fixpoint flatten_contract (c : Contract) : list Contract :=
+match c with
+| c0 _+_ c1 => (flatten_contract c0) ++ (flatten_contract c1)
+| _ => [c]
+end.
+
+Definition aci_eq (c0 c1 : Contract) : bool :=
+ let c0_l := flatten_contract c0 in
+ let c1_l := flatten_contract c1 in
+ (inclb c0_l c1_l) && (inclb c1_l c0_l) .
+
+Definition aci_p_eq (p0 p1: (Contract * Contract)) : bool :=
+ let (c0,c0') := p0 in
+ let (c1,c1') := p1 in
+ aci_eq c0 c1 && aci_eq c0' c1'.*)
+
+(*
+Fixpoint trace_derive (c: Contract) (s : Trace) :=
+match s with
+| [] => c
+| e::s' => trace_derive (c/e) s'
+end.*)
+
+
+
+
+
+
+(*Maybe keep*)
+Lemma finitely_many_derivatives : forall c, exists (l : list Contract), (forall s, member aci_eq (trace_derive c s) l = true).
+Proof. Admitted.
+
+
+Global Opaque alphabet.
+Definition direct_derivatives (c : Contract) : list Contract := map (fun e => c/e) alphabet.
+
+
+
+
+
+
+Definition direct_p_derivatives (p : Contract * Contract) : list (Contract * Contract) := 
+ map (fun e => ((fst p) / e,(snd p) / e)) alphabet.
+(*processed contract -> all direct derivatives are in either internal_nodes or leafs
+  not processed contract -> no direct derivatives in either internal_nodes or leafs*)
+Definition p_derivative_closure_once (l_pair : (list (Contract*Contract)) * (list (Contract * Contract))) :=
+ let (internal_nodes,leafs) := l_pair in
+ let internal_nodes' := internal_nodes++leafs in
+ let leaf_children := flat_map direct_p_derivatives leafs
+ in (internal_nodes',filter (fun c => negb (member aci_p_eq c internal_nodes')) leaf_children).
+
+Definition approx_p_derivative_closure (n : nat) (p : (Contract * Contract)) :=
+ approx n p_derivative_closure_once ([],[p]).
+
+
+(*All internal_nodes and leafs share the property that they can be derived from trace_derive c s
+  with some trace s. Only new derivatives are placed in leafs, and finitely_many_derivatives states
+  that there are only finitely many of those, therefore at some point, this list will be empty
+  in which case a fixpoint has been reached*)
+Lemma p_derivative_closure_convergence : forall (c0 c1 : Contract), exists (n:nat),
+ approx_p_derivative_closure n (c0,c1) =  approx_p_derivative_closure (n+1) (c0,c1). 
+Proof. Admitted.
+
+Definition p_derivative_relation (arg_rec arg_inp : list (Contract*Contract) * list (Contract*Contract)) :=
+  p_derivative_closure_once arg_inp <> arg_inp /\  (*Not converged*)
+  p_derivative_closure_once arg_inp = arg_rec. (*is preceeding element*)
+
+Lemma well_founded_p_derivative_relation: well_founded p_derivative_relation.
+Proof. Admitted.
+
+Instance wf_p_derivative_relation : WellFounded p_derivative_relation := well_founded_p_derivative_relation.
+
+Lemma list_not_eq : forall (A:Type) (l0 l1 : list A) (p : A), l0++p::l1 = l0 -> False.
+Proof.
+intro. induction l0;intros.
+- discriminate.
+- inversion H. eauto. 
+Qed.
+
+
+Lemma cons_i_not_convergence : forall (p : Contract*Contract)(internal_nodes leafs : list (Contract*Contract)),
+   p_derivative_closure_once (internal_nodes,p::leafs) <> (internal_nodes,p::leafs).
+Proof.
+intros. simpl. intro H. injection H. intros.
+eauto using list_not_eq.
+Qed.
+
+Equations p_derivative_closure (internal_nodes_leafs : list (Contract*Contract) * list (Contract*Contract)) : list (Contract*Contract) by  wf internal_nodes_leafs p_derivative_relation :=
+p_derivative_closure (internal_nodes, []) := internal_nodes;
+p_derivative_closure (internal_nodes, leafs) := p_derivative_closure (p_derivative_closure_once (internal_nodes, leafs)).
+Next Obligation.
+unfold p_derivative_relation. split.
+- apply cons_i_not_convergence.
+- auto.
+Qed.
+Global Transparent p_derivative_closure.
+
+
+Definition derivative_closure (c0 c1 : Contract) : list (Contract*Contract) := p_derivative_closure ([],[(c0,c1)]).
+
+
+(*Show lemma that all derivatives are in derivative_closure*)
+Lemma derivative_closure_is_bisimulation : forall (c0 c1 : Contract), 
+ Forall (fun (p : Contract * Contract) => nu (fst p) = nu (snd p)) (derivative_closure c0 c1) -> bisimulation (fun x y => (In (x,y) (derivative_closure c0 c1))).
+Proof. Admitted.
+
+Definition decide_contract_equivalence (c0 c1 : Contract) := 
+ forallb (fun (p : Contract * Contract) => eqb (nu (fst p)) (nu (snd p)) ) (derivative_closure c0 c1).
+
+Lemma Bisimilarity_reflect : forall (c0 c1 : Contract), reflect (Bisimilarity c0 c1) (decide_contract_equivalence c0 c1).
+Proof. Admitted.
+
+
+
